comex

lunarlander_sl/newParallel.thy
@@ -17,22 +17,25 @@ inductive in_inv_assn :: "(gstate \<Rightarrow> bool) \<Rightarrow> (gstate \<Ri
 inductive io_inv_assn :: "(gstate \<Rightarrow>  bool) \<Rightarrow> (gstate \<Rightarrow> real \<Rightarrow> bool) \<Rightarrow> cname \<Rightarrow> tassn" ("IOinv\<^sub>t") where
   "r s  \<Longrightarrow> g s v \<Longrightarrow> IOinv\<^sub>t r g ch [IOBlock ch v]"
 
-inductive wait_inv_assn :: "(gstate \<Rightarrow>  bool) \<Rightarrow> rdy_info \<Rightarrow> tassn" ("Waitinv\<^sub>t") where
-  " Waitinv\<^sub>t r rdy []"
-| "d > 0 \<Longrightarrow> (\<forall>t\<in>{0..d}. r (p t)) \<Longrightarrow> Waitinv\<^sub>t r rdy [WaitBlk (ereal d) p rdy]" 
+inductive wait_inv_assn :: "(gstate \<Rightarrow> real \<Rightarrow> bool) \<Rightarrow> (real \<Rightarrow> bool) \<Rightarrow> rdy_info \<Rightarrow> tassn" ("Waitinv\<^sub>t") where
+  "Waitinv\<^sub>t r dp rdy []"
+| "d > 0 \<Longrightarrow> dp d \<Longrightarrow> (\<forall>t\<in>{0..d}. r (p t) t) \<Longrightarrow> Waitinv\<^sub>t r dp rdy [WaitBlk (ereal d) p rdy]" 
 
 
-inductive s2gs1 :: "(state \<Rightarrow> bool) \<Rightarrow> (gstate \<Rightarrow> bool)" where
- "p s \<Longrightarrow> s2gs1 p (State s)"
+inductive sb2gsb :: "(state \<Rightarrow> bool) \<Rightarrow> (gstate \<Rightarrow> bool)" where
+ "p s \<Longrightarrow> sb2gsb p (State s)"
 
-inductive s2gs2 :: "(state \<Rightarrow> real \<Rightarrow> bool) \<Rightarrow> (gstate \<Rightarrow> real \<Rightarrow> bool)" where
- "p s v \<Longrightarrow> s2gs2 p (State s) v"
+inductive srb2gsrb :: "(state \<Rightarrow> real \<Rightarrow> bool) \<Rightarrow> (gstate \<Rightarrow> real \<Rightarrow> bool)" where
+ "p s v \<Longrightarrow> srb2gsrb p (State s) v"
 
-inductive pgs2gs1 :: "(gstate \<Rightarrow> bool) \<Rightarrow> (gstate \<Rightarrow> bool) \<Rightarrow> (gstate \<Rightarrow> bool)" where
- "r1 s \<Longrightarrow> r2 s' \<Longrightarrow> pgs2gs1 r1 r2 (ParState s s') "
+inductive pgsb2gsb :: "(gstate \<Rightarrow> bool) \<Rightarrow> (gstate \<Rightarrow> bool) \<Rightarrow> (gstate \<Rightarrow> bool)" where
+ "r1 s \<Longrightarrow> r2 s' \<Longrightarrow> pgsb2gsb r1 r2 (ParState s s') "
 
-inductive pgs2gs2 :: "(gstate \<Rightarrow> real \<Rightarrow> bool) \<Rightarrow> (gstate \<Rightarrow> real \<Rightarrow> bool) \<Rightarrow> (gstate \<Rightarrow> real \<Rightarrow> bool)" where
- "r1 s v \<Longrightarrow> r2 s' v \<Longrightarrow> pgs2gs2 r1 r2 (ParState s s') v"
+inductive pgsrb2gsrb :: "(gstate \<Rightarrow> real \<Rightarrow> bool) \<Rightarrow> (gstate \<Rightarrow> real \<Rightarrow> bool) \<Rightarrow> (gstate \<Rightarrow> real \<Rightarrow> bool)" where
+ "r1 s v \<Longrightarrow> r2 s' v \<Longrightarrow> pgsrb2gsrb r1 r2 (ParState s s') v"
+
+inductive gsb2gsrb :: "(gstate \<Rightarrow> bool) \<Rightarrow> (gstate \<Rightarrow> real \<Rightarrow> bool)" where
+ "r s \<Longrightarrow> gsb2gsrb r s t"
 
 lemma combine_assn_emp_ininv:
   "ch \<in> chs \<Longrightarrow> combine_assn chs emp\<^sub>t (Ininv\<^sub>t r g ch @\<^sub>t P) = false\<^sub>A"
@@ -51,44 +54,45 @@ lemma combine_assn_emp_outinv:
 lemma combine_assn_ininv_outinv:
   "ch \<in> chs \<Longrightarrow>
    combine_assn chs (Ininv\<^sub>t r1 g1 ch @\<^sub>t P) (Outinv\<^sub>t r2 g2 ch @\<^sub>t Q) \<Longrightarrow>\<^sub>t
-   (IOinv\<^sub>t (pgs2gs1 r1 r2) (pgs2gs2 g1 g2) ch @\<^sub>t combine_assn chs P Q)"
+   (IOinv\<^sub>t (pgsb2gsb r1 r2) (pgsrb2gsrb g1 g2) ch @\<^sub>t combine_assn chs P Q)"
   unfolding combine_assn_def
   apply (auto simp add: entails_tassn_def join_assn_def pure_assn_def conj_assn_def io_inv_assn.simps
-                        out_inv_assn.simps in_inv_assn.simps pgs2gs1.simps pgs2gs2.simps)
+                        out_inv_assn.simps in_inv_assn.simps pgsb2gsb.simps pgsrb2gsrb.simps)
   apply (auto elim: sync_elims)
   by (metis append_Cons append_self_conv2 combine_blocks_pairE)
 
 lemma combine_assn_emp_waitinv:
-  "combine_assn chs emp\<^sub>t (Waitinv\<^sub>t p rdy @\<^sub>t P) \<Longrightarrow>\<^sub>t combine_assn chs emp\<^sub>t P"
+  "combine_assn chs emp\<^sub>t (Waitinv\<^sub>t  p dp rdy @\<^sub>t P) \<Longrightarrow>\<^sub>t combine_assn chs emp\<^sub>t P"
   unfolding combine_assn_def
-  apply (auto simp add: entails_tassn_def wait_inv_assn.simps emp_assn_def join_assn_def false_assn_def)
+  apply (auto simp add: entails_tassn_def wait_inv_assn.simps emp_assn_def 
+join_assn_def false_assn_def)
   by (auto elim: sync_elims)
 
 
-lemma combine_assn_wait_in:
+lemma combine_assn_waitinv_ininv:
   assumes "ch \<in> chs"
     and "compat_rdy rdy1 ({}, {ch})"
-  shows "combine_assn chs (Waitinv\<^sub>t r1 rdy1 @\<^sub>t P) (Ininv\<^sub>t r2 g ch @\<^sub>t Q) \<Longrightarrow>\<^sub>t
-   (Waitinv\<^sub>t (pgs2gs1 r1 r2) (merge_rdy rdy1 ({}, {ch})) @\<^sub>t
+  shows "combine_assn chs (Waitinv\<^sub>t r1 dp rdy1 @\<^sub>t P) (Ininv\<^sub>t r2 g ch @\<^sub>t Q) \<Longrightarrow>\<^sub>t
+   (Waitinv\<^sub>t (pgsrb2gsrb r1 (gsb2gsrb r2)) dp (merge_rdy rdy1 ({}, {ch})) @\<^sub>t
     combine_assn chs P (Ininv\<^sub>t r2 g ch @\<^sub>t Q))"
 proof-
-  have *:"(Waitinv\<^sub>t (pgs2gs1 r1 r2) (merge_rdy rdy1 ({}, {ch})) @\<^sub>t
+  have *:"(Waitinv\<^sub>t (pgsrb2gsrb r1 (gsb2gsrb r2)) dp (merge_rdy rdy1 ({}, {ch})) @\<^sub>t
     combine_assn chs P (Ininv\<^sub>t r2 g ch @\<^sub>t Q)) tr" if
-        "(Waitinv\<^sub>t r1 rdy1 @\<^sub>t P) tr1" "(Ininv\<^sub>t r2 g ch @\<^sub>t Q) tr2" 
+        "(Waitinv\<^sub>t r1 dp rdy1 @\<^sub>t P) tr1" "(Ininv\<^sub>t r2 g ch @\<^sub>t Q) tr2" 
         "combine_blocks chs tr1 tr2 tr" for tr tr1 tr2
   proof-
     from that(1)[unfolded join_assn_def]
-    obtain tr11 tr12 where a: "Waitinv\<^sub>t r1 rdy1 tr11" "P tr12" "tr1 = tr11 @ tr12"
+    obtain tr11 tr12 where a: "Waitinv\<^sub>t r1 dp rdy1 tr11" "P tr12" "tr1 = tr11 @ tr12"
       by auto
     from that(2)[unfolded join_assn_def]
     obtain tr21 tr22 where b: "Ininv\<^sub>t r2 g ch tr21" "Q tr22" "tr2 = tr21 @ tr22"
       by auto
-    have d:"(Waitinv\<^sub>t (pgs2gs1 r1 r2) (merge_rdy rdy1 ({}, {ch})) @\<^sub>t
+    have d:"(Waitinv\<^sub>t (pgsrb2gsrb r1 (gsb2gsrb r2)) dp (merge_rdy rdy1 ({}, {ch})) @\<^sub>t
      combine_assn chs P (Ininv\<^sub>t r2 g ch @\<^sub>t Q)) tr" if 
-        "0 < d2" "0<d"
+        "0 < d2" "0<d" "dp d"
         "combine_blocks chs (WaitBlk (ereal d) p rdy1 # tr12)
           (WaitBlk (ereal d2) (\<lambda>_. s) ({}, {ch}) # InBlock ch v # tr22) tr" 
-        "\<forall>t\<in>{0..d}. r1 (p t)"
+        "\<forall>t\<in>{0..d}. r1 (p t) t"
         "r2 s "  "g s v "
       for d p s v d2
     proof -
@@ -99,7 +103,7 @@ proof-
         have d1': "ereal d < ereal d2"
           using d1 by auto
         show ?thesis
-          using that(3)
+          using that(4)
           apply (elim combine_blocks_waitE3)
              apply (rule that(2)) apply (rule d1') using assms(2) apply simp
           subgoal for blks'
@@ -108,7 +112,7 @@ proof-
             apply (rule exI[where x=blks'])
             apply (rule conjI)
             subgoal 
-              apply(auto simp add:wait_inv_assn.simps pgs2gs1.simps)
+              apply(auto simp add:wait_inv_assn.simps pgsrb2gsrb.simps gsb2gsrb.simps)
               apply(rule exI[where x="d"])
               apply(rule exI[where x="(\<lambda>t. ParState (p t) s)"])
               using that by auto
@@ -129,7 +133,7 @@ proof-
       next
         assume d2: "d = d2"
         show ?thesis
-          using that(3) unfolding d2[symmetric]
+          using that(4) unfolding d2[symmetric]
           apply (elim combine_blocks_waitE2)
           using assms(2) apply simp
           subgoal for blks'
@@ -137,7 +141,7 @@ proof-
             apply (rule exI[where x="[WaitBlk d (\<lambda>t. ParState (p t) s) (merge_rdy rdy1 ({}, {ch}))]"])
             apply (rule exI[where x=blks'])
             apply (rule conjI)
-            subgoal using that apply (auto simp add: wait_inv_assn.simps pgs2gs1.simps)
+            subgoal using that apply (auto simp add: wait_inv_assn.simps pgsrb2gsrb.simps gsb2gsrb.simps)
               by blast
             apply (rule conjI)
              prefer 2 subgoal by auto
@@ -158,7 +162,7 @@ proof-
         have d3': "ereal d > ereal d2"
           using d3  by auto
         show ?thesis
-          using that(3)
+          using that(4)
           apply (elim combine_blocks_waitE4)
           apply (rule that(1)) apply (rule d3')
            using assms(2) apply simp
@@ -166,11 +170,11 @@ proof-
           using assms by auto
       qed
         qed
-      have e: "(Waitinv\<^sub>t (pgs2gs1 r1 r2) (merge_rdy rdy1 ({}, {ch})) @\<^sub>t
+      have e: "(Waitinv\<^sub>t (pgsrb2gsrb r1 (gsb2gsrb r2)) dp (merge_rdy rdy1 ({}, {ch})) @\<^sub>t
      combine_assn chs P (Ininv\<^sub>t r2 g ch @\<^sub>t Q)) tr" if 
         "combine_blocks chs (WaitBlk (ereal d) p rdy1 # tr12)
-          (WaitBlk \<infinity> (\<lambda>_. s) ({}, {ch}) # tr22) tr" "0 < d " 
-          "\<forall>t\<in>{0..d}. r1 (p t)" "r2 s" for d p s
+          (WaitBlk \<infinity> (\<lambda>_. s) ({}, {ch}) # tr22) tr" "0 < d " "dp d" 
+          "\<forall>t\<in>{0..d}. r1 (p t) t" "r2 s" for d p s
       proof -
       have e1: "\<infinity> - ereal d = \<infinity>"
         by auto
@@ -183,7 +187,7 @@ proof-
           apply (rule exI[where x="[WaitBlk d (\<lambda>t. ParState (p t) s) (merge_rdy rdy1 ({}, {ch}))]"])
           apply (rule exI[where x=blks'])
           apply (rule conjI)
-            subgoal apply(simp add: wait_inv_assn.simps pgs2gs1.simps) by blast
+            subgoal apply(simp add: wait_inv_assn.simps pgsrb2gsrb.simps gsb2gsrb.simps) by blast
             apply (rule conjI)
              prefer 2 apply simp
             unfolding combine_assn_def
